Test/civl/samples/bluetooth.bpl
@@ -16,7 +16,7 @@ datatype Perm { Left(i: int), Right(i: int) }
 
 var {:layer 0,3} stoppingFlag: bool;
 var {:layer 0,2} stopped: bool;
-var {:layer 1,2} {:linear} usersInDriver: Set Perm;
+var {:layer 1,2} {:linear} usersInDriver: Set (One Perm);
 var {:layer 0,1} pendingIo: int;
 var {:layer 0,1} stoppingEvent: bool;
 
@@ -27,13 +27,18 @@ yield invariant {:layer 1} Inv1();
 preserves stoppingEvent ==> stoppingFlag && usersInDriver->val == MapConst(false);
 preserves pendingIo == Set_Size(usersInDriver) + (if stoppingFlag then 0 else 1);
 
+function {:inline} Split(i: int, l: Set (One Perm), r: Set (One Perm)): bool
+{
+    l == Set_Singleton(One(Left(i))) && r == Set_Singleton(One(Right(i)))
+}
+
 // user code
 
 yield procedure {:layer 2}
-User(i: int, {:layer 1,2} {:linear} l: Set Perm, {:linear} {:layer 1,2} r: Set Perm)
+User(i: int, {:layer 1,2} {:linear} l: Set (One Perm), {:linear} {:layer 1,2} r: Set (One Perm))
 preserves call Inv2();
 preserves call Inv1();
-requires {:layer 1, 2} l->val == MapOne(Left(i)) && r->val == MapOne(Right(i));
+requires {:layer 1, 2} Split(i, l, r);
 {
     while (*)
     invariant {:yields} true;
@@ -46,52 +51,52 @@ requires {:layer 1, 2} l->val == MapOne(Left(i)) && r->val == MapOne(Right(i));
     }
 }
 
-atomic action {:layer 2} AtomicEnter#1(i: int, {:linear_in} l: Set Perm, {:linear} r: Set Perm)
+atomic action {:layer 2} AtomicEnter#1(i: int, {:linear_in} l: Set (One Perm), {:linear} r: Set (One Perm))
 modifies usersInDriver;
 {
     assume !stoppingFlag;
     call Set_Put(usersInDriver, l);
 }
 yield procedure {:layer 1}
-Enter#1(i: int, {:layer 1} {:linear_in} l: Set Perm, {:layer 1} {:linear} r: Set Perm)
+Enter#1(i: int, {:layer 1} {:linear_in} l: Set (One Perm), {:layer 1} {:linear} r: Set (One Perm))
 refines AtomicEnter#1;
 preserves call Inv1();
-requires {:layer 1} l->val == MapOne(Left(i)) && r->val == MapOne(Right(i));
+requires {:layer 1} Split(i, l, r);
 {
     call Enter();
     call {:layer 1} usersInDriver := A(usersInDriver, l);
 }
 
-pure action A({:linear_in} usersInDriver: Set Perm, {:linear_in} l: Set Perm)
-  returns ({:linear} usersInDriver': Set Perm)
+pure action A({:linear_in} usersInDriver: Set (One Perm), {:linear_in} l: Set (One Perm))
+  returns ({:linear} usersInDriver': Set (One Perm))
 {
     usersInDriver' := usersInDriver;
     call Set_Put(usersInDriver', l);
 }
 
-left action {:layer 2} AtomicCheckAssert#1(i: int, {:linear} r: Set Perm)
+left action {:layer 2} AtomicCheckAssert#1(i: int, {:linear} r: Set (One Perm))
 {
-    assert r->val == MapOne(Right(i)) && usersInDriver->val[Left(i)];
+    assert r == Set_Singleton(One(Right(i))) && Set_Contains(usersInDriver, One(Left(i)));
     assert !stopped;
 }
 yield procedure {:layer 1}
-CheckAssert#1(i: int, {:layer 1} {:linear} r: Set Perm)
+CheckAssert#1(i: int, {:layer 1} {:linear} r: Set (One Perm))
 refines AtomicCheckAssert#1;
 preserves call Inv1();
 {
     call CheckAssert();
 }
 
-left action {:layer 2} AtomicExit(i: int, {:linear_out} l: Set Perm, {:linear} r: Set Perm)
+left action {:layer 2} AtomicExit(i: int, {:linear_out} l: Set (One Perm), {:linear} r: Set (One Perm))
 modifies usersInDriver;
 {
-    assert l->val == MapOne(Left(i)) && r->val == MapOne(Right(i));
+    assert Split(i, l, r);
     call usersInDriver := B(usersInDriver, l);
 }
 yield procedure {:layer 1}
-Exit(i: int, {:layer 1} {:linear_out} l: Set Perm, {:layer 1} {:linear} r: Set Perm)
+Exit(i: int, {:layer 1} {:linear_out} l: Set (One Perm), {:layer 1} {:linear} r: Set (One Perm))
 refines AtomicExit;
-requires {:layer 1} l->val == MapOne(Left(i)) && r->val == MapOne(Right(i));
+requires {:layer 1} Split(i, l, r);
 preserves call Inv1();
 {
     call DeleteReference();
@@ -99,8 +104,8 @@ preserves call Inv1();
     call {:layer 1} Lemma_SetSize_Subset(Set_Empty(), usersInDriver);
 }
 
-pure action B({:linear_in} usersInDriver: Set Perm, {:linear_out} l: Set Perm)
-  returns ({:linear} usersInDriver': Set Perm)
+pure action B({:linear_in} usersInDriver: Set (One Perm), {:linear_out} l: Set (One Perm))
+  returns ({:linear} usersInDriver': Set (One Perm))
 {
     assert Set_IsSubset(l, usersInDriver);
     usersInDriver' := usersInDriver;
