Test/civl/regression-tests/linear-types-fail.bpl
@@ -24,12 +24,12 @@ procedure P4(a: int) returns ({:linear} a': int) {
     a' := a;
 }
 
-procedure P5({:linear} a: Set int, {:linear_in} b: One int) {
+procedure P5({:linear} a: Set (One int), {:linear_in} b: One int) {
     call One_Put(a, b);
 }
 
-procedure P6({:linear_in} a: Set int, {:linear} b: One int) {
-    var {:linear} a': Set int;
+procedure P6({:linear_in} a: Set (One int), {:linear} b: One int) {
+    var {:linear} a': Set (One int);
     a' := a;
     call One_Put(a', b);
 }
